## 3.3.3 Expected Value of a Linear Function 

The $h\left( X\right)$ function of interest is quite frequently a linear
function ${aX} + b$ . In this case,
$E\left\lbrack {h\left( X\right) }\right\rbrack$ is easily computed from
$E\left( X\right)$ without the need for additional summation.

$$E\left( {{aX} + b}\right) = a \cdot E\left( X\right) + b$$

::: mdframed
PROPOSITION
:::

(Or, using alternative notation,
${\mu }_{{aX} + b} = a \cdot {\mu }_{X} + b$ )

To paraphrase, the expected value of a linear function equals the linear
function evaluated at the expected value $E\left( X\right)$ . Since
$h\left( X\right)$ in Example 3.23 is linear and
$E\left( X\right) = 2,E\left\lbrack {h\left( X\right) }\right\rbrack = {800}\left( 2\right) - {900} = \$ {700}$
, as before.

Proof

$$E\left( {{aX} + b}\right) = \mathop{\sum }\limits_{D}\left( {{ax} + b}\right) \cdot p\left( x\right) = a\mathop{\sum }\limits_{D}x \cdot p\left( x\right) + b\mathop{\sum }\limits_{D}p\left( x\right)$$

$$= {aE}\left( X\right) + b$$

Two special cases of the proposition yield two important rules of
expected value.

1\. For any constant $a,E\left( {aX}\right) = a \cdot E\left( X\right)$
(take $b = 0$ ).(3.12)

2\. For any constant $b,E\left( {X + b}\right) = E\left( X\right) + b$
(take $a = 1$ ).

Multiplication of $X$ by a constant $a$ typically changes the unit of
measurement, for example, from inches to $\mathrm{{cm}}$ , where
$a = {2.54}$ . Rule 1 says that the expected value in the new units
equals the expected value in the old units multiplied by the conversion
factor $a$ . Similarly, if a constant $b$ is added to each possible
value of $X$ , then the expected value will be shifted by that same
constant amount.