> [!question]
> 1. 已知 $\boldsymbol{A}=\left(\begin{array}{ll}2 & 0 \\ 0 & 3\end{array}\right)$, 则 $A^{-1}=\left(\begin{array}{ll}\frac{1}{2} & 0 \\ 0 & \frac{1}{3}\end{array}\right)$.
> 2. 设 $\boldsymbol{A}=\left(\begin{array}{ll}2 & 1 \\ 0 & 3\end{array}\right)$ ，求其逆矩阵。

解 
(1) 由定义验算即得.
(2) 设 $\boldsymbol{B}=\left(\begin{array}{ll}b_{1} & b_{2} \\ b_{3} & b_{4}\end{array}\right)$ 是 $\boldsymbol{A}$ 的逆矩阵, 则
$$
\left(\begin{array}{ll}
2 & 1 \\
0 & 3
\end{array}\right)\left(\begin{array}{ll}
b_{1} & b_{2} \\
b_{3} & b_{4}
\end{array}\right)=\left(\begin{array}{ll}
1 & 0 \\
0 & 1
\end{array}\right)
$$

那么
$$
\left\{\begin{aligned}
2 b_{1}+b_{3} & =1 \\
2 b_{2}+b_{4} & =0 \\
3 b_{3} & =0 \\
3 b_{4} & =1
\end{aligned}\right.
$$

解得 $b_{1}=\frac{1}{2}, b_{2}=-\frac{1}{6}, b_{3}=0, b_{4}=\frac{1}{3}$, 即 $\boldsymbol{A}^{-1}=\left(\begin{array}{rr}\frac{1}{2} & -\frac{1}{6} \\ 0 & \frac{1}{3}\end{array}\right)$.