# 例 2.29 
已知 ${\mathbf{A}}^{ * } = \left( \begin{matrix} 1 & - 2 & 1 \\ 0 & 2 & - 2 \\ - 1 & 2 & 1 \end{matrix}\right)$ ,求 $\mathbf{A}$ .

解 计算 ${\mathbf{A}}^{ * }$ 的行列式可得 $\left| {\mathbf{A}}^{ * }\right| = 4$ . 因为 $\left| {\mathbf{A}}^{ * }\right| = {\left| \mathbf{A}\right| }^{n - 1}$ ,得 ${\left| \mathbf{A}\right| }^{2} = 4$ , $\left| \mathbf{A}\right| = \pm 2$ .

若 $\left| \mathbf{A}\right| = 2$ ,由 ${\mathbf{A}}^{ * } = \left| \mathbf{A}\right| {\mathbf{A}}^{-1}$ 得

$$
{\mathbf{A}}^{-1} = \frac{1}{2}{\mathbf{A}}^{ * } = \left( \begin{matrix} \frac{1}{2} & - 1 & \frac{1}{2} \\ 0 & 1 & - 1 \\ - \frac{1}{2} & 1 & \frac{1}{2} \end{matrix}\right)
$$

于是

$$
\mathbf{A} = {\left( {\mathbf{A}}^{-1}\right) }^{-1} = \left( \begin{array}{lll} 3 & 2 & 1 \\ 1 & 1 & 1 \\ 1 & 0 & 1 \end{array}\right)
$$

若 $\left| \mathbf{A}\right| = - 2$ ,则 ${\mathbf{A}}^{-1} = - \frac{1}{2}{\mathbf{A}}^{ * }$ ,故

$$
\mathbf{A} = \left( \begin{matrix} - 3 & - 2 & - 1 \\ - 1 & - 1 & - 1 \\ - 1 & 0 & - 1 \end{matrix}\right) .\square \tag{口}
$$