# 例 2.24
设 $A, B$ 为 $n$ 阶矩阵,求证: ${\left( AB\right) }^{ * } = {B}^{ * }{A}^{ * }$ .

证明 设 $\mathbf{C} = \mathbf{A}\mathbf{B}$ . 记 ${M}_{ij},{N}_{ij},{P}_{ij}$ 分别是 $\mathbf{A},\mathbf{B},\mathbf{C}$ 中第 $\left( {i, j}\right)$ 元素的余子式, ${A}_{ij},{B}_{ij},{C}_{ij}$ 分别是 $\mathbf{A},\mathbf{B},\mathbf{C}$ 中第 $\left( {i, j}\right)$ 元素的代数余子式. 注意到

$$
{\mathbf{A}}^{ * } = \left( \begin{matrix} {A}_{11} & {A}_{21} & \cdots & {A}_{n1} \\ {A}_{12} & {A}_{22} & \cdots & {A}_{n2} \\ \vdots & \vdots & & \vdots \\ {A}_{1n} & {A}_{2n} & \cdots & {A}_{nn} \end{matrix}\right) ,\;{\mathbf{B}}^{ * } = \left( \begin{matrix} {B}_{11} & {B}_{21} & \cdots & {B}_{n1} \\ {B}_{12} & {B}_{22} & \cdots & {B}_{n2} \\ \vdots & \vdots & & \vdots \\ {B}_{1n} & {B}_{2n} & \cdots & {B}_{nn} \end{matrix}\right)
$$

${\mathbf{B}}^{ * }{\mathbf{A}}^{ * }$ 的第 $\left( {i, j}\right)$ 元素为

$$
\mathop{\sum }\limits_{{k = 1}}^{n}{B}_{ki}{A}_{jk}
$$

而 ${\mathbf{C}}^{ * }$ 的第 $\left( {i, j}\right)$ 元素就是 ${C}_{ji} = {\left( -1\right) }^{j + i}{P}_{ji}$ . 由 Cauchy-Binet 公式可得

$$
{C}_{ji} = {\left( -1\right) }^{j + i}{P}_{ji} = {\left( -1\right) }^{j + i}\mathop{\sum }\limits_{{k = 1}}^{n}{M}_{jk}{N}_{ki}
$$

$$
= \mathop{\sum }\limits_{{k = 1}}^{n}{\left( -1\right) }^{j + k}{M}_{jk}{\left( -1\right) }^{i + k}{N}_{ki} = \mathop{\sum }\limits_{{k = 1}}^{n}{A}_{jk}{B}_{ki},
$$

故结论成立.